Dpda/HopcroftToCPSP.lean
@@ -8,11 +8,198 @@ def Hopcroft_DPDA_IDesc.toCPSP {Q S Γ} [Fintype Q] [DecidableEq Q] [Fintype S /
   (pwβ: Hopcroft_DPDA_IDesc Q S Γ) : CPSP_DPDA_IDesc (AugmentOneState Q) S Γ :=
   ⟨AugmentOneState.fromQ pwβ.p, pwβ.w, pwβ.β⟩
 
-theorem Hopcroft_to_CPSP_preserves_semantics_single_step {Q S Γ}
+def Hopcroft_DPDA.toCPSP {Q S Γ} [DecidableEq Q] [DecidableEq Γ] (M: Hopcroft_DPDA Q S Γ) : CPSP_DPDA (AugmentOneState Q) S Γ :=
+  let q_neg1 : AugmentOneState Q := AugmentOneState.qNeg1
+  let F : Finset (AugmentOneState Q) := Finset.image (fun (q: Q) => AugmentOneState.fromQ q) M.pda.F
+  let new_transition : CPSP_Transition (AugmentOneState Q) S Γ := fun ⟨q', X⟩ =>
+    match q', X with
+    | AugmentOneState.qNeg1, .z0 =>
+      CPSP_Judge.immediate (some
+        (M.pda.z0 :: [], AugmentOneState.fromQ M.pda.q0)
+      ) -- protect the stack bottom
+    | AugmentOneState.qNeg1, .fromΓ _ => CPSP_Judge.immediate none -- stack shall be empty at the start
+    | AugmentOneState.fromQ _, .z0 => CPSP_Judge.immediate none -- stack shall never be empty later
+    | AugmentOneState.fromQ q, .fromΓ x => Hopcroft_DPDA.Δ M ⟨q, x⟩
+  ⟨q_neg1, F, new_transition⟩
+
+theorem Hopcroft_to_CPSP_preserves_semantics_single_step_when_stack_bottom_is_protected {Q S Γ}
   [Fintype Q] [DecidableEq Q] [Fintype S /- Σ -/] [Fintype Γ] [DecidableEq Γ]
-  (M: Hopcroft_DPDA Q S Γ) (idesc: Hopcroft_DPDA_IDesc Q S Γ) :
+  (M: Hopcroft_DPDA Q S Γ) (idesc: Hopcroft_DPDA_IDesc Q S Γ) (stack_bottom_protected: ∃ s, idesc.β = s ++ [M.pda.z0]) :
   let M_cpsp : CPSP_DPDA (AugmentOneState Q) S Γ := Hopcroft_DPDA.toCPSP M
   let idesc_cpsp := Hopcroft_DPDA_IDesc.toCPSP idesc
   let after_step : Option (Hopcroft_DPDA_IDesc Q S Γ) := Hopcroft_DPDA.stepTransition M idesc
   let after_step_cpsp : Option (CPSP_DPDA_IDesc (AugmentOneState Q) S Γ) := CPSP_Judge.stepTransition M_cpsp.transition idesc_cpsp
-  after_step.map Hopcroft_DPDA_IDesc.toCPSP = after_step_cpsp := sorry
+  after_step.map Hopcroft_DPDA_IDesc.toCPSP = after_step_cpsp := by
+  simp only [
+    Hopcroft_DPDA_IDesc.toCPSP,
+    Hopcroft_DPDA.toCPSP,
+    Hopcroft_DPDA.stepTransition,
+    CPSP_Judge.stepTransition
+  ]
+  cases h : idesc.β with
+  | nil => simp /- However, this case is absurd under our assumption -/
+  | cons A γ =>
+    simp [h]
+    cases h2 : M.Δ (idesc.p, A) with
+    | step f =>
+      simp [h2]
+      cases h3 : idesc.w with
+      | nil =>
+        simp [h3]
+        unfold Hopcroft_PreDPDA.transition
+        match h4 : M.pda.4 (idesc.p, none, A) with
+        | none =>
+          simp [h4]
+        | some (p, α) =>
+          simp [h4]
+          unfold Hopcroft_DPDA.Δ at h2
+          simp at h2
+          rw [h4] at h2
+          simp at h2
+      | cons head tail =>
+        simp [h3]
+        match f head with
+        | none =>
+          simp
+          unfold Hopcroft_DPDA.Δ at h2
+          match h4 : M.pda.transition (idesc.p, none, A) with
+          | some (p, α) =>
+            simp [Option.map_some, Option.some.injEq]
+            simp at h2
+            rw [h4] at h2
+            simp at h2
+          | none =>
+            simp
+            match h5 : M.pda.transition (idesc.p, some head, A) with
+            | none =>
+              simp
+            | some (p2, α2) =>
+              simp [h5]
+              have h6 := M.deterministic
+              sorry
+        | some val =>
+          unfold Hopcroft_DPDA_IDesc.toCPSP
+          simp
+          match h4 : M.pda.transition (idesc.p, none, A) with
+          | some (p, α) =>
+            simp
+            unfold Hopcroft_DPDA.Δ at h2
+            simp at h2
+            rw [h4] at h2
+            simp at h2
+          | none =>
+            simp
+            sorry
+    | immediate a =>
+      cases h3 : idesc.w with
+      | nil =>
+        simp [h3]
+        unfold Hopcroft_PreDPDA.transition
+        match h4 : M.pda.transition (idesc.p, none, A) with
+        | some (p, α) =>
+          simp [h4]
+          unfold Hopcroft_DPDA_IDesc.toCPSP
+          simp
+          unfold Hopcroft_DPDA.Δ at h2
+          match a with
+          | none =>
+            simp
+            simp at h2
+            rw [h4] at h2
+            simp at h2
+          | some (p2, α2) =>
+            simp at h2
+            rw [h4] at h2
+            simp at h2
+            obtain ⟨ u, v ⟩ := h2
+            simp
+            exact ⟨ v, u ⟩
+        | none =>
+          simp [h4]
+          match a with
+          | none =>
+            simp
+          | some (p2, α2) =>
+            simp
+            unfold Hopcroft_DPDA.Δ at h2
+            simp at h2
+            rw [h4] at h2
+            simp at h2
+      | cons head tail =>
+        simp [h3]
+        match h4 : CPSP_Judge.immediate a with
+        | CPSP_Judge.step b2 =>
+          simp [h4]
+          unfold Hopcroft_PreDPDA.transition
+          cases b2 head with
+          | none =>
+            simp
+            match h5 : M.pda.transition (idesc.p, none, A) with
+            | some (p, α) =>
+              simp [h5]
+              contradiction
+            | none =>
+              simp [h5]
+              match h6 : M.pda.transition (idesc.p, some head, A) with
+              | none =>
+                simp [h6]
+              | some (p2, α2) =>
+                simp [h6]
+                contradiction
+          | some u =>
+            simp
+            match h5 : M.pda.4 (idesc.p, none, A) with
+            | none =>
+              simp [h5]
+              contradiction
+            | some (p, α) =>
+              contradiction
+        | CPSP_Judge.immediate a2 =>
+          unfold Hopcroft_DPDA_IDesc.toCPSP
+          unfold Hopcroft_DPDA.Δ at h2
+          simp at h2
+          match h5 : M.pda.transition (idesc.p, none, A) with
+          | some (p, α) =>
+            simp
+            match a2 with
+            | some (u, v) =>
+              simp [h5]
+              rw [h5] at h2
+              simp at h2
+              unfold Hopcroft_PreDPDA.transition at h5
+              simp at h4
+              rw [← h2] at h4
+              simp at h4
+              exact ⟨ h4.right, h4.left ⟩
+            | none =>
+              simp at h4
+              rw [h4] at h2
+              rw [h5] at h2
+              simp at h2
+          | none =>
+            simp
+            match M.pda.transition (idesc.p, some head, A) with
+            | some (p, α) =>
+              simp
+              rw [← h4, ← h2, h5]
+              simp
+              match M.pda.transition (idesc.p, some head, A) with
+              | some (p2, α2) =>
+                simp
+                rw [h5] at h2
+                simp at h2
+              | none =>
+                simp
+                rw [h5] at h2
+                simp at h2
+            | none =>
+              simp
+              rw [← h4, ← h2, h5]
+              simp
+              match M.pda.transition (idesc.p, some head, A) with
+              | some (p2, α2) =>
+                simp
+                rw [h5] at h2
+                simp at h2
+              | none =>
+                simp
